Move a new version of generic RO with the corresponding eager proof. Should help a lot in the proof of squeezeless sponge and also in the Alley part.

sha3/proof/old/MyRO.ec
@@ -1,5 +1,39 @@
 require import Option List FSet NewFMap.
-        import NewLogic.
+        import NewLogic Fun.
+
+(* TODO: move this *)
+lemma set_eq (m:('a,'b)fmap) x y: m.[x] = Some y => m.[x<-y] = m.
+proof.
+  by rewrite fmapP=> Hx x';rewrite getP;case (x'=x)=>//->;rewrite Hx.
+qed.
+
+lemma oflistK_uniq (s : 'a list) : uniq s =>
+  perm_eq s (elems (oflist s)).
+proof. by move/undup_id => {1}<-; apply/FSet.oflistK. qed.
+
+lemma setD1E (s : 'a fset) x :
+  perm_eq (elems (s `\` fset1 x)) (rem x (elems s)).
+proof.
+rewrite setDE; pose s' := List.filter _ _; apply/(perm_eq_trans s').
+  rewrite perm_eq_sym oflistK_uniq ?filter_uniq ?uniq_elems.
+rewrite /s' rem_filter ?uniq_elems; apply/uniq_perm_eq;
+  rewrite ?filter_uniq ?uniq_elems // => y.
+by rewrite !mem_filter /predC in_fset1.
+qed.
+
+lemma perm_to_rem (s:'a fset) x : 
+  mem s x => perm_eq (elems s) (x :: elems (s `\` fset1 x)).
+proof.
+rewrite memE => /perm_to_rem /perm_eqlP->; apply/perm_cons.
+have /perm_eqlP <- := (setD1E s x); rewrite perm_eq_refl.
+qed.
+
+lemma mem_drop (s:'a list) n x: mem (drop n s) x => mem s x.
+proof. by rewrite -{2}(cat_take_drop n) mem_cat=>->. qed.
+
+lemma mem_take (s:'a list) n x: mem (take n s) x => mem s x.
+proof. by rewrite -{2}(cat_take_drop n) mem_cat=>->. qed.
+(* end TODO *)
 
 abstract theory Titer.
 
@@ -17,6 +51,14 @@ module Iter (O:Orcl) = {
     }
   }
 }.
+
+lemma iter_ll(O<:Orcl): islossless O.f => islossless Iter(O).iter.
+proof.
+  move=> O_ll;proc;inline Iter(O).iter.
+  while true (size l);auto=>/=.
+  + call O_ll;skip=> /=?[*]Hl<-;smt ml=0 w=(size_eq0 size_ge0 size_drop).
+  smt ml=0 w=(size_eq0 size_ge0).  
+qed.
 
 section.
 
@@ -36,7 +78,7 @@ proof.
      ={glob O})
     (l{1}= i' :: i :: (s1 ++ s2) /\ l{2} = i' :: (s1 ++ i::s2) /\ ={glob O} ==>
      ={glob O})=>//.
-  + by move=> ?&ml[*]<*>;exists (glob O){ml}, (i' :: i :: (s1 ++ s2)).
+  + by move=> ?&mr[*]<*>;exists (glob O){mr}, (i' :: i :: (s1 ++ s2)).
   + proc;rcondt{1}1=>//;rcondt{2}1=>//.
     rcondt{1}3;1:by auto;conseq(_: true).
     rcondt{2}3;1:by auto;conseq(_: true).
@@ -45,7 +87,7 @@ proof.
       (l{1} = i :: i' :: (s1 ++ s2) /\ ={l, glob O} ==> ={l,glob O})
       (l{1} = i :: i' :: (s1 ++ s2) /\ 
        l{2} = i' :: i :: (s1 ++ s2) /\  ={glob O} ==> ={l,glob O})=>//.
-    + by move=>?&ml[*]<*>;exists (glob O){ml}, (i :: i' :: (s1 ++ s2)).
+    + by move=>?&mr[*]<*>;exists (glob O){mr}, (i :: i' :: (s1 ++ s2)).
     + inline *;rcondt{2} 2;1:by auto. 
       rcondt{2} 4;1:by auto;sp;conseq(_:true).
       rcondf{2} 6; auto;call(_:true);wp;call(_:true);auto.
@@ -53,7 +95,7 @@ proof.
       (l{1} = i :: i' :: (s1 ++ s2) /\ 
        l{2} = i' :: i :: (s1 ++ s2) /\  ={glob O} ==> ={l,glob O})
       (l{2} = i' :: i :: (s1 ++ s2) /\ ={l, glob O} ==> ={l,glob O})=>//.
-    + by move=>?&ml[*]<*>;exists (glob O){ml}, (i' :: i :: (s1 ++ s2)).
+    + by move=>?&mr[*]<*>;exists (glob O){mr}, (i' :: i :: (s1 ++ s2)).
     + wp; by call (iter_swap1 i i').
       (* call iter_swap1: FIXME catch exception *)
     inline *;rcondt{1} 2;1:by auto. 
@@ -65,12 +107,12 @@ proof.
   transitivity{1} {Iter(O).iter(l); }
    (={l,glob O} /\ l{1}= i::(s1++s2) ==> ={glob O})
    (={glob O} /\ l{1}=i::(s1++s2) /\ l{2}= (s1++i::s2) ==> ={glob O})=>//.
-  + by move=>?&ml[*]<*>;exists (glob O){ml}, (i :: (s1 ++ s2)).
+  + by move=>?&mr[*]<*>;exists (glob O){mr}, (i :: (s1 ++ s2)).
   + by inline *;sim.    
   transitivity{1} {Iter(O).iter(l); }
    (={glob O} /\ l{1}=i::(s1++s2) /\ l{2}= (s1++i::s2) ==> ={glob O})
    (={l,glob O} /\ l{2}= (s1++i::s2) ==> ={glob O})=>//.
-  + by move=>?&ml[*]<*>;exists (glob O){ml}, (s1 ++ i::s2).
+  + by move=>?&mr[*]<*>;exists (glob O){mr}, (s1 ++ i::s2).
   + by call Hrec;auto.
   by inline*;sim.         
 qed.
@@ -88,19 +130,19 @@ proof.
   transitivity Iter(O).iter 
     (l{1}=i::s1 /\ l{2}=i::(s3++s4) /\ ={glob O} ==> ={glob O})
     (l{1}=i::(s3++s4) /\ l{2}=s3++i::s4 /\ ={glob O} ==> ={glob O})=>//.
-  + by move=>?&ml[*]-> -> _ ->; exists (glob O){ml}, (i :: (s3 ++ s4)).
+  + by move=>?&mr[*]-> -> _ ->; exists (glob O){mr}, (i :: (s3 ++ s4)).
   + proc;rcondt{1}1=>//;rcondt{2}1=>//.
     seq 2 2: (s1 = l{1} /\ l{2}=s3++s4 /\ ={glob O}).
     + by wp;call(_:true);auto;progress;rewrite drop0.
     transitivity{1} {Iter(O).iter(l); }
       (={l,glob O} ==> ={glob O}) 
       (s1 = l{1} /\ l{2} = s3 ++ s4 /\ ={glob O} ==> ={glob O})=>//.
-    + by move=>?&ml[*]-> -> ->;exists (glob O){ml}, l{1}.
+    + by move=>?&mr[*]-> -> ->;exists (glob O){mr}, l{1}.
     + by inline Iter(O).iter;sim.
     transitivity{1} {Iter(O).iter(l); }
       (s1 = l{1} /\ l{2} = s3 ++ s4 /\ ={glob O} ==> ={glob O})
       (={l,glob O} ==> ={glob O}) =>//.
-    + by move=>?&ml[*]-> -> ->;exists (glob O){ml}, (s3++s4).
+    + by move=>?&mr[*]-> -> ->;exists (glob O){mr}, (s3++s4).
     + move: eq_s12; rewrite -(cat1s i s4) catA perm_eq_sym.
       rewrite perm_catCA /= perm_cons perm_eq_sym=> Hp.
     + call (ih (s3++s4) Hp)=>//.
@@ -155,14 +197,29 @@ proof.
   by rewrite oget_some /=;case (f' = f)=> [_ ->|].
 qed.
 
-lemma restr_set_diff f2 f1 m x y: 
+lemma restr_set m f1 f2 x y: 
+  restr f1 m.[x<-(y,f2)] = if f1 = f2 then (restr f1 m).[x<-y] else rem x (restr f1 m).
+proof.
+  rewrite fmapP;case (f1=f2)=>[->|Hneq]x0;rewrite !(restrP,getP);1: by case (x0=x).
+  case (x0=x)=>[->|Hnx];1:by rewrite (eq_sym f2) Hneq remP_eq.
+  by rewrite remP Hnx restrP.
+qed.
+
+lemma restr_set_eq m f x y: 
+  restr f m.[x<-(y,f)] = (restr f m).[x<-y].
+proof. by rewrite restr_set. qed.
+
+lemma restr0 f : restr f map0 = map0.
+proof. by apply fmapP=>x;rewrite restrP !map0P. qed.
+
+lemma restr_set_neq f2 f1 m x y: 
   !mem (dom m) x =>
   f2 <> f1 => restr f1 m.[x<-(y,f2)] = restr f1 m.
 proof.
-  rewrite fmapP in_dom=>/= Hdom Hf x';rewrite !restrP getP.
-  by case (x' = x)=>//=->;rewrite Hf Hdom.
+  by move=>Hm Hneq;rewrite restr_set (eq_sym f1) Hneq rem_id//restr_dom Hm.
 qed.
 
+(* -------------------------------------------------------------------------- *)
 module RO : RO = {
   var m : (from, to * flag)fmap
 
@@ -221,6 +278,8 @@ end section LL.
  
 end Ideal.
 
+
+(* -------------------------------------------------------------------------- *)
 abstract theory GenEager.
 
 clone include Ideal. 
@@ -260,9 +319,32 @@ module ERO : RO = {
 
 }.
 
-lemma set_eq (m:('a,'b)fmap) x y: m.[x] = Some y => m.[x<-y] = m.
+lemma resample_ll : islossless ERO.resample.
+proof. 
+  proc;call (iter_ll ERO.I _)=>//;apply (sample_ll sampleto_ll).
+qed.
+
+lemma eager_init :
+  eager [ERO.resample(); , RO.init ~ ERO.init, ERO.resample(); :
+         ={RO.m} ==> ={RO.m} ].
 proof.
-  by rewrite fmapP=> Hx x';rewrite getP;case (x'=x)=>//->;rewrite Hx.
+  eager proc. inline{2} *;rcondf{2}3;auto=>/=.
+  + by move=>?_;rewrite restr0 dom0 elems_fset0.
+  by conseq (_:) (_:true==>true: =1%r) _=>//;call resample_ll.
+qed.
+
+lemma iter_perm2 (i1 i2 : from):
+  equiv[ Iter(ERO.I).iter ~ Iter(ERO.I).iter :
+          l{1} = [i1; i2] /\ l{2} = [i2; i1] /\ ={glob ERO.I} ==>
+          ={glob ERO.I}].
+proof.
+  proc;rcondt{1}1=>//;rcondt{2}1=>//.
+  rcondt{1}3;1:by auto;conseq(_:true).
+  rcondt{2}3;1:by auto;conseq(_:true).
+  seq 4 4 : (={l,RO.m});2:by sim.
+  case (i1=i2);1:by sim.
+  inline *;swap[4..5]-2;swap{2} 6-2;auto=>?&mr[*]3!<*>Hneq/=?->?->/=.
+  by rewrite set_set Hneq. 
 qed.
 
 lemma eager_get :
@@ -274,7 +356,7 @@ proof.
   + rnd{1};rcondf{2} 2;1:by auto=> /#.
     alias{1} 1 mx = oget RO.m.[x];inline *.
     while (={l,RO.m} /\ (!mem l x /\ RO.m.[x] = Some (mx.`1,Known)){1}).
-    + auto=>?&ml[*]-> ->;case (l{ml})=>//=x2 l2 Hmx Hgx?->.
+    + auto=>?&mr[*]-> ->;case (l{mr})=>//=x2 l2 Hmx Hgx?->.
       by rewrite getP drop0 /#.
     auto=>??[*]-> ->/= Hmem HK;rewrite sampleto_ll/==> r _. 
     rewrite -memE restr_dom Hmem/= HK.
@@ -282,722 +364,200 @@ proof.
     by move=>????-> _[*]_-> _ Heq?;rewrite in_dom set_eq Heq. 
   rcondt{2} 2. + auto=> ?[*]-> ->;rewrite negb_and /#.
   case ((mem (dom RO.m) x){1}).
-  + inline{1} ERO.resample=>/=.
+  + inline{1} ERO.resample=>/=;rnd{1}.
     transitivity{1} { Iter(ERO.I).iter(x::elems ((dom (restr Unknown RO.m)) `\` fset1 x));
-                      r <$ sampleto x; }
+                      }
       (={x,RO.m} /\ mem (dom RO.m{1}) x{1} /\ (oget RO.m{1}.[x{1}]).`2 = Unknown ==>
        ={x,RO.m})
       (={x,RO.m} /\ mem (dom RO.m{1}) x{1} /\ (oget RO.m{1}.[x{1}]).`2 = Unknown==>
        ={x} /\ eq_except RO.m{1} RO.m{2} (fset1 x{1}) /\
        RO.m{1}.[x{2}] = Some (result{2},Unknown) /\
        RO.m{2}.[x{2}] = Some (result{2},Known)).
-    + by move=>?&ml[*]-> -> ??;exists RO.m{ml}, x{ml}=>/#.
+    + by move=>?&mr[*]-> -> ??;exists RO.m{mr}, x{mr}=>/#.
     + move=>???;rewrite in_dom=>[*]<*>[*]->/eq_except_sym H Hxm Hx2.
-      rewrite Hxm oget_some /=;apply /eq_sym.
+      rewrite sampleto_ll=> r _;rewrite /= Hxm oget_some /=;apply /eq_sym.
       have /(congr1 oget):= Hx2 => <-;apply eq_except_set_eq=>//.
       by rewrite in_dom Hx2.
-    + rnd;call (iter_perm ERO.I _).
-
-  
-
-
-
-      cut ->: (result{2}, Known) = oget RO.m{2}.[x{2}]. 
-        
-
-      search eq_except.
- set_eq.
- 1:Hx.
-;rewrite H=>{H}.    
-
- <- ((oget RO.m{1}.[x{1}]).`1, Known)] = RO.m{2}
-     mem (dom RO.m{1} x{1}
-
-    transitivity{1} { work <- dom RO.m;
-                      r <$ sampleto x;
-                      while (work <> fset0) {
-                        x0  <- pick work;
-                        if (in_dom_with RO.m x0 Unknown) {
-                          c   <$ sampleto x0;
-                          RO.m.[x0] <- (if x0 = x then r else c, Unknown);
-                        }
-                        work <- work `\` fset1 (pick work);
-                      } }
-      (={x,RO.m} ==> ={x,RO.m})
-      (={x,RO.m} /\ (mem (dom RO.m) x /\ (oget RO.m.[x]).`2 = Unknown){1} ==>
-       ={x} /\ RO.m{1} = RO.m{2}.[x{2}<-(result{2}, Unknown)] /\ 
-       RO.m{2}.[x{2}] = Some(result{2}, Known)).
-    + move=>?&mr[*]-> ->??;exists RO.m{mr},x{mr}=>/#.
-    + move=>?&m?[2*]-> -> <- ->_. 
-      by rewrite in_dom getP_eq oget_some set_set set_eq.
-    + seq 1 1:(={work,x,RO.m});[by sim|symmetry]. 
-      eager while (H:r<$sampleto x; ~ r<$sampleto x; : ={x} ==> ={r})=>//;1,3:by sim.
-      swap{1}2-1;sp 1 1.
-      if{2};[rcondt{1}2|rcondf{1}2];1,3,4:by auto.
-      by rnd{2};wp;case ((x0 = x){1});[rnd{1}|];auto=>??[*]-> -> -> -> ->_ _ _->;
-         rewrite sampleto_ll.
-    alias{1} 1 cx = (oget RO.m.[x]).`1.
-    while (={work,x,r} /\ mem (dom RO.m{1}) x{1} /\ (RO.m.[x]=Some(r,Known)){2}/\
-               RO.m{1} = (RO.m.[x<-(if mem work x then cx{1} else r, Unknown)]){2}).
-    + sp 1 1;case ((x0 = x){1}).
-      + rcondt{1} 1. by auto;progress;rewrite getP_eq oget_some;case (mem _ _).
-        rcondf{2} 1. by auto=> @/in_dom_with;progress;rewrite H0. 
-        auto=> ??[*]_-> -> -> ->?-> ->?_<-/=;rewrite sampleto_ll=>c _.
-        by rewrite dom_set !inE /= set_set.
-      if=>//. auto;progress[-split]. by rewrite /in_dom_with dom_set getP !inE H3.
-      + auto;progress [-split];split=>// _.
-        by rewrite dom_set !inE H/= getP set_set (eq_sym x{2}) H3 H0.
-      by auto;progress;rewrite !inE (eq_sym x{2}) H3.
-    auto;progress [-split];rewrite H1 /=.
-    rewrite dom_set fsetUC subset_fsetU_id /=.
-    + by move=> x;rewrite inE.
-    rewrite H getP_eq /= set_set /= set_eq. 
-    + by rewrite {1}get_oget // -H0;case (oget _).
-    by move=> ????-> ->/=[*];rewrite !inE oget_some. 
-  inline *;swap{1} 3 -2.
-  admit.
-(*
-  (* Admit *)
-  while (={work,x,r} /\ (RO.m.[x]=None){1} /\ 
-         RO.m{2} = RO.m{1}.[x{2}<-(r{2},Known)] /\
-         !mem work{2} x{2}).
-  + wp;sp 1 1;if. auto=> ??[*]-> -> -> Hex Hmem Heq Hx _ /= ?->/=.
-    rewrite !inE Hmem !getP Heq /=.
-    cut ^Hd->/=: x{2} <> pick work{2} by smt ml=0 w=mem_pick.
-    by rewrite Hex set_set Hd.
-  auto=>??/=[*]-> -> _ ^Hdom;rewrite in_dom=>/=Hnone?->;rewrite restr_set_diff//=.
-  by rewrite Hnone /= restr_dom Hdom=>????-> ->[*];rewrite in_dom getP_eq. *)
+    + call (iter_perm ERO.I iter_perm2).
+      skip=> &1 &2 [[->> ->>]] [Hdom Hm];progress.
+      by apply /perm_to_rem/restr_dom;rewrite Hdom Hm.
+    inline *;rcondt{1} 2;1:by auto.
+    while (={x,l} /\ !mem l{1} x{1}/\
+           eq_except RO.m{1} RO.m{2} (fset1 x{1}) /\
+           RO.m{1}.[x{2}] = Some (result{2}, Unknown) /\
+           RO.m{2}.[x{2}] = Some (result{2}, Known)).
+    + auto=> ?&mr[*]2!->Hm Hex Hm1 Hmr Hneq _/=?->.
+      rewrite (contra _ _ (mem_drop _ 1 _) Hm) /=.
+      rewrite!getP;move:Hm;rewrite-(mem_head_behead witness l{mr})//negb_or=>-[]->_.
+      by rewrite Hm1 Hmr/=;apply eq_except_set. 
+    auto=>?&mr[[->>->>]][]Hdom Hm /=/=?->/=.
+    rewrite !drop0 restr_set /= dom_rem /= -memE !inE /=.
+    by rewrite !getP_eq /= oget_some/= set2_eq_except.
+  inline *. swap{1}3-2.
+  while (={l,x} /\ !mem l{1} x{1} /\ RO.m{1}.[x{1}] = None /\
+         RO.m{2} = RO.m{1}.[x{2}<-(r{2},Known)]).
+  + auto=> ?&mr[*]2!->Hm Hn Heq Hl _/=?->.
+    rewrite (contra _ _ (mem_drop _ 1 _) Hm) /=.
+    rewrite set_set -Heq !getP -(eq_sym (x{mr})).
+    by move:Hm;rewrite -(mem_head_behead witness l{mr} Hl) -Hn negb_or=>-[]->.
+  auto=> ?&mr[*]2!->_ Hnm/=?->.
+  rewrite -memE restr_set_neq //= restr_dom Hnm /=.
+  by have:=Hnm;rewrite in_dom/==>->/=????->->;rewrite in_dom getP_eq oget_some. 
 qed.
- 
-search "_.[_<-_]".
-    search 
-  auto=> ??/=[*]-> -> _ Hmem/=?->/=;rewrite restr_set_diff //=.
-  rewrite eq_except_sym set_eq_except restr_dom Hmem getP_eq=>????->_ [*].
 
-  rewrite Hmem.
-
- get_eq.
-
-  transitivity{2} {
-  
-=>-[->//|/#].
-
-
- {1}(get_oget m_R x{2}).
-print get_oget.
-search "_.[_]" "_.[_<-_]".
-print restrK.
-
-
-smt.
- H /=;smt. 
-  case ((!mem work x){1}).
-  + swap{1} 2 -1;while (={work,x} /\ eq_except RO.m{1} RO.m{2} (fset1 x{1}) /\ 
-                         (!mem work x){1} /\ (RO.m.[x] = Some rd){2} /\ (!mem (dom RO.m) x){1}). 
-    + inline *;auto;progress [-split].
-      cut -> : mem (dom RO.m{2}) (pick work{2}) = mem (dom RO.m{1}) (pick work{2}) by rewrite !in_dom;smt.
-      smt. 
-    auto;progress [-split];rewrite !getP_eq;smt. 
-  inline RO.f.
-  transitivity{1} { rd <$ sample x;
-                    while (work <> fset0) {
-                      x0  <- pick work;
-                      rd0 <$ sample x0;
-                      if (!mem (dom RO.m) x0)
-                        RO.m.[x0] <- if x0 = x then rd else rd0;
-                      work <- work `\` fset1 (pick work);
-                    } }
-     (={x,work,RO.m} ==> ={x,RO.m})
-     ((={x,work,RO.m} /\ mem work{1} x{1}) /\ ! mem (dom RO.m{2}) x{2} ==>
-           ={x,RO.m} /\ (result = oget RO.m.[x]){2} /\ mem (dom RO.m{1}) x{1}) => //.
-  + by move=> &1 &2 H; exists RO.m{2}, x{2}, work{2}; move: H.
-  + transitivity{1} { while (work <> fset0) {
-                        x0  <- pick work;
-                        rd0 <$ sample x0;
-                        if (!mem (dom RO.m) x0) RO.m.[x0] <- rd0;
-                        work <- work `\` fset1 (pick work);
+lemma eager_set :
+  eager [ERO.resample(); , RO.set ~ ERO.set, ERO.resample(); :
+         ={x,y} /\ ={RO.m} ==> ={res,RO.m} ].
+proof.
+  eager proc.
+  case ((mem (dom RO.m) x /\ (oget RO.m.[x]).`2 = Unknown){1}).
+  inline{1} ERO.resample=>/=;wp 1 2.
+    transitivity{1} { Iter(ERO.I).iter(x::elems ((dom (restr Unknown RO.m)) `\` fset1 x));
                       }
-                      rd <$ sample x; }
-        (={x,work,RO.m} ==> ={x,RO.m})
-        (={x,work,RO.m} ==> ={x,RO.m})=> //.
-    + by move=> &1 &2 H; exists RO.m{2}, x{2}, work{2}; move: H.
-    + by sim; rnd{2}; sim : (={x,IND_Eager.H.m}); smt.
-    symmetry; eager while (H: rd <$ sample x; ~ rd <$ sample x; : ={x} ==> ={rd})=> //; sim. 
-    swap{2} 5 -4; swap [2..3] -1; case ((x = pick work){1}).
-    + by wp; rnd{2}; rnd; rnd{1}; wp; skip; smt.
-    by auto; smt.
-  + while (={x, work} /\
-           (!mem work x => mem (dom RO.m) x){1} /\
-            RO.m.[x]{2} = Some rd{1} /\
-            if (mem (dom RO.m) x){1} then ={RO.m}
-            else eq_except RO.m{1} RO.m{2} (fset1 x{1})).
-    + auto;progress; 1..9,12:smt.
-      + case ((pick work = x){2})=> pick_x; last smt.
-        subst x{2}; move: H7 H1; rewrite -neqF /eq_except=> -> /= eq_exc.
-        by apply fmapP=> x0; case (pick work{2} = x0); smt.
-    by auto; smt.
-  by auto;progress [-split];rewrite H0 /= getP_eq;smt. 
+      (={x,y,RO.m} /\ mem (dom RO.m{1}) x{1} /\ (oget RO.m{1}.[x{1}]).`2 = Unknown ==>
+       ={x,y,RO.m})
+      (={x,y,RO.m} /\ mem (dom RO.m{1}) x{1} /\ (oget RO.m{1}.[x{1}]).`2 = Unknown==>
+       ={x,y} /\ eq_except RO.m{1} RO.m{2} (fset1 x{1}) /\
+       RO.m{2}.[x{2}] = Some (y{2},Known)).
+    + by move=>?&mr[*]-> -> ???;exists RO.m{mr}, y{mr}, x{mr}=>/#.
+    + move=>??? [*]<*>[*]-> -> Hex Hm2.
+      by rewrite (eq_except_set_eq RO.m{2} RO.m{m} x{2}) ?in_dom ?Hm2// eq_except_sym.
+    + call (iter_perm ERO.I iter_perm2).
+      skip=>?&mr[][]->>[]->>->>[]Hdom Hm/=.
+      by apply /perm_to_rem/restr_dom;rewrite Hdom Hm.
+    inline *;rcondt{1} 2;1:by auto.
+    while (={x,l} /\ !mem l{1} x{1}/\
+           eq_except RO.m{1} RO.m{2} (fset1 x{1}) /\
+           RO.m{2}.[x{2}] = Some (y{2}, Known)).
+    + auto=> ?&mr[*]2!->Hm Hex Hm1 Hmr _/=?->.
+      rewrite (contra _ _ (mem_drop _ 1 _) Hm) /=.
+      rewrite!getP;move:Hm;rewrite-(mem_head_behead witness l{mr})//negb_or=>-[]->_.
+      by rewrite Hm1 /=;apply eq_except_set. 
+    auto=>?&mr[*]3!<*>Hdom Hm /=/=;rewrite !drop0 sampleto_ll=>/=?_.
+    by rewrite -memE restr_set /= dom_rem !inE !getP_eq set2_eq_except.
+  inline *;wp.
+  while (={x,l} /\ !mem l{1} x{1}/\
+         eq_except RO.m{1} RO.m{2} (fset1 x{1}) /\
+         RO.m{2}.[x{2}] = Some (y{2}, Known)).
+  + auto=> ?&mr[*]2!->Hm Hex Hm1 Hmr _/=?->.
+    rewrite (contra _ _ (mem_drop _ 1 _) Hm) /=.
+    rewrite!getP;move:Hm;rewrite-(mem_head_behead witness l{mr})//negb_or=>-[]->_.
+    by rewrite Hm1 /=;apply eq_except_set. 
+  auto=> ?&mr[*]3!-> Hnm /=. 
+  rewrite-memE restr_set/=rem_id?restr_dom//=Hnm.
+  rewrite getP_eq eq_except_sym set_eq_except/=.
+  move=>/=????2!->/=[]/eq_except_sym? Hx2;apply/eq_sym.
+  have/(congr1 oget):=Hx2=><-;apply eq_except_set_eq=>//;by rewrite in_dom Hx2.
+qed.
 
+lemma eager_in_dom:
+  eager [ERO.resample(); , RO.in_dom ~ ERO.in_dom, ERO.resample(); :
+         ={x,f} /\ ={RO.m} ==> ={res,RO.m} ].
+proof.
+  eager proc;inline *;wp.
+  while (={l,RO.m} /\ (forall z, mem l z => in_dom_with RO.m z Unknown){1} /\
+         in_dom_with RO.m{1} x{1} f{1} = result{2}).
+  + auto=>?&mr[*]2!->Hz <-?_/=?->/=. 
+    by split=>[z Hm|];rewrite /in_dom_with dom_set getP !inE/#.
+  by auto=>?&mr/=[*]3!->/=;split=>// z;rewrite -memE restr_dom. 
+qed.
 
+lemma eager_restrK:
+  eager [ERO.resample(); , RO.restrK ~ ERO.restrK, ERO.resample(); :
+         ={RO.m} ==> ={res,RO.m} ].
+proof.
+  eager proc;inline *;wp.
+  while (={l,RO.m} /\ (forall z, mem l z => in_dom_with RO.m z Unknown){1} /\
+         restr Known RO.m{1} = result{2}).
+  + auto=>?&mr[*]2!->Hz<-?_/=?->/=. 
+    split=>[z Hm|];1:by rewrite /in_dom_with dom_set getP !inE/#.
+    rewrite restr_set rem_id?restr_dom//.
+    by move:H=>/(mem_head_behead witness) /(_ (head witness l{mr})) /= /Hz /#.
+  by auto=>?&mr/=->/=;split=>// z;rewrite -memE restr_dom. 
+qed.
 
+lemma eager_sample:
+  eager [ERO.resample(); , RO.sample ~ ERO.sample, ERO.resample(); :
+         ={x,RO.m} ==> ={res,RO.m} ].
+proof.
+  eager proc.
+  transitivity{2} {
+      c <$ sampleto x; RO.m.[x] <- (c, Unknown);
+      Iter(ERO.I).iter(x::elems ((dom (restr Unknown RO.m)) `\` fset1 x));}
+      (={x,RO.m} ==> ={x,RO.m}) 
+      (={x,RO.m} ==> ={x,RO.m})=>//;last first.
+  + inline{2} ERO.resample;call (iter_perm ERO.I iter_perm2);auto=>?&mr[]->->/=?->.
+    by rewrite !restr_set/= !dom_set perm_eq_sym perm_to_rem !inE.
+  + by move=>?&mr[*]2!->;exists RO.m{mr}, x{mr}.
+  inline ERO.resample;inline{2}*;rcondt{2}4;1:by auto.
+  wp;case ((!mem (dom RO.m) x \/ (oget RO.m.[x]).`2=Known){1}).
+  + inline *;swap{1}3-1.
+    while (={x,l} /\ RO.m{1}.[x{1} <- (c{1}, Unknown)] = RO.m{2} /\ !(mem l x){1}).
+    + auto=>?&mr[*]2!-><- Hnm Hl _/=?->.
+      rewrite (contra _ _ (mem_drop _ 1 _) Hnm) /= set_set.
+      by move:Hnm;rewrite-(mem_head_behead witness l{mr})//negb_or eq_sym=>-[]->.
+    auto=>?&mr[*]2!->?/=;rewrite sampleto_ll=>?_?->;rewrite drop0.
+    rewrite restr_set/= dom_set fsetDK.
+    cut<-/=:dom (restr Unknown RO.m{mr}) =
+            dom (restr Unknown RO.m{mr}) `\` fset1 x{mr}.
+    + apply fsetP=>z;rewrite !(restr_dom,inE)/#.
+    by rewrite set_set/= -memE restr_dom;split=>/#.
+  transitivity{1} {
+    Iter(ERO.I).iter(x::elems ((dom (restr Unknown RO.m)) `\` fset1 x));
+    c<$ sampleto x;}
+    (={x,RO.m} /\ (mem (dom RO.m) x /\ (oget RO.m.[x]).`2=Unknown){1} ==> ={x,c,RO.m}) 
+    (={x,RO.m} /\ (mem (dom RO.m) x /\ (oget RO.m.[x]).`2=Unknown){1} ==> 
+     ={x} /\ RO.m{1}.[x{1} <- (c{1}, Unknown)] = RO.m{2})=>//.
+  + by move=>?&mr[*]2!->?;exists RO.m{mr}, x{mr}=>/#.
+  + rnd;call (iter_perm ERO.I iter_perm2);auto=>?&mr[*]->->/=??;split=>//.
+    by rewrite perm_to_rem restr_dom.
+  inline *;rcondt{1}2;1:by auto.
+  swap{1} 7-2.
+  while (={x,l} /\ RO.m{1}.[x{1} <- (c{1}, Unknown)] = RO.m{2} /\ !(mem l x){1}).
+  + auto=>?&mr[*]2!-><- Hnm Hl _/=?->.
+    rewrite (contra _ _ (mem_drop _ 1 _) Hnm) /= set_set.
+    by move:Hnm;rewrite-(mem_head_behead witness l{mr})//negb_or eq_sym=>-[]->.
+  by auto=>?&mr[*]2!->??/=?->?->;rewrite!drop0 restr_set/=dom_set fsetDK-memE!inE.
+qed.
 
+module Eager (D:Distinguisher) = {
 
-
-
-
-
-
-
-
-
-  module IND_S(D:Distinguisher) = {
-    proc main(): bool = {
-      var b;
-      RO.init();
-      b <@ D(RO).distinguish();
-      ERO.sample();
-      return b;
-    }  
-  }.
-
-  section EAGER.
-
-    local lemma eager_query:
-       eager [ERO.sample(); , RO.f ~ ERO.f, ERO.sample(); :
-                 ={x,RO.m} ==> ={res,RO.m} ].
-    proof.
-      eager proc.
-      inline ERO.sample;swap{2} 4 -3.
-      seq 1 1: (={x,work,RO.m});first by sim.
-      wp;case ((mem (dom RO.m) x){1}).
-      + rnd{1}.
-        alias{1} 1 mx = oget RO.m.[x].
-        while (={work,RO.m} /\ (RO.m.[x] = Some mx){1}). 
-        + by inline *;auto;progress;smt.
-        auto;progress [- split]; rewrite sample_ll H /=;smt. 
-      case ((!mem work x){1}).
-      + swap{1} 2 -1;while (={work,x} /\ eq_except RO.m{1} RO.m{2} (fset1 x{1}) /\ 
-                             (!mem work x){1} /\ (RO.m.[x] = Some rd){2} /\ (!mem (dom RO.m) x){1}). 
-        + inline *;auto;progress [-split].
-          cut -> : mem (dom RO.m{2}) (pick work{2}) = mem (dom RO.m{1}) (pick work{2}) by rewrite !in_dom;smt.
-          smt. 
-        auto;progress [-split];rewrite !getP_eq;smt. 
-      inline RO.f.
-      transitivity{1} { rd <$ sample x;
-                        while (work <> fset0) {
-                          x0  <- pick work;
-                          rd0 <$ sample x0;
-                          if (!mem (dom RO.m) x0)
-                            RO.m.[x0] <- if x0 = x then rd else rd0;
-                          work <- work `\` fset1 (pick work);
-                        } }
-         (={x,work,RO.m} ==> ={x,RO.m})
-         ((={x,work,RO.m} /\ mem work{1} x{1}) /\ ! mem (dom RO.m{2}) x{2} ==>
-               ={x,RO.m} /\ (result = oget RO.m.[x]){2} /\ mem (dom RO.m{1}) x{1}) => //.
-      + by move=> &1 &2 H; exists RO.m{2}, x{2}, work{2}; move: H.
-      + transitivity{1} { while (work <> fset0) {
-                            x0  <- pick work;
-                            rd0 <$ sample x0;
-                            if (!mem (dom RO.m) x0) RO.m.[x0] <- rd0;
-                            work <- work `\` fset1 (pick work);
-                          }
-                          rd <$ sample x; }
-            (={x,work,RO.m} ==> ={x,RO.m})
-            (={x,work,RO.m} ==> ={x,RO.m})=> //.
-        + by move=> &1 &2 H; exists RO.m{2}, x{2}, work{2}; move: H.
-        + by sim; rnd{2}; sim : (={x,IND_Eager.H.m}); smt.
-        symmetry; eager while (H: rd <$ sample x; ~ rd <$ sample x; : ={x} ==> ={rd})=> //; sim. 
-        swap{2} 5 -4; swap [2..3] -1; case ((x = pick work){1}).
-        + by wp; rnd{2}; rnd; rnd{1}; wp; skip; smt.
-        by auto; smt.
-      + while (={x, work} /\
-               (!mem work x => mem (dom RO.m) x){1} /\
-                RO.m.[x]{2} = Some rd{1} /\
-                if (mem (dom RO.m) x){1} then ={RO.m}
-                else eq_except RO.m{1} RO.m{2} (fset1 x{1})).
-        + auto;progress; 1..9,12:smt.
-          + case ((pick work = x){2})=> pick_x; last smt.
-            subst x{2}; move: H7 H1; rewrite -neqF /eq_except=> -> /= eq_exc.
-            by apply fmapP=> x0; case (pick work{2} = x0); smt.
-        by auto; smt.
-      by auto;progress [-split];rewrite H0 /= getP_eq;smt. 
-    qed.
-
-    equiv Eager_S (D <: Distinguisher{RO}): IND_S(D).main ~ IND(ERO,D).main: ={glob D} ==> ={res,RO.m,glob D}.
-    proof.
-      proc; inline ERO.init RO.init.
-      seq 1 1: (={glob D, RO.m});first by wp. 
-      symmetry; eager (H: ERO.sample(); ~ ERO.sample();: ={RO.m} ==> ={RO.m}): 
-            (={glob D, RO.m}) => //; first by sim.
-      eager proc H (={RO.m}) => //; [by apply eager_query | by sim].
-    qed.
-
-    equiv Eager (D <: Distinguisher{RO}): IND(RO,D).main ~ IND(ERO,D).main: ={glob D} ==> ={res,glob D}.
-    proof.
-      transitivity IND_S(D).main
-          (={glob D} ==> ={res,glob D})
-          (={glob D} ==> ={res,RO.m,glob D}) => //.
-      + by progress;exists (glob D){2}.
-      + proc;inline{2} ERO.sample.
-        while{2} true (card work{2}). 
-        + move=> &m1 z;wp;call (f_ll sample_ll);auto;smt.
-        conseq (_: _ ==> ={b,glob D}) => //;[smt | by sim].
-      apply (Eager_S D).
-    qed.
-
-  end section EAGER.
-
-end GenIdeal.
-
-
-
-
-
-
-
-
-
-
-
-
-
-
-
-abstract theory 
-
-
-module type SAMPLE = {
-  proc sampleI(h:handle) : unit
-  proc setD(h:handle, c:capacity) : unit
-  proc get(h:handle) : capacity
-  proc in_dom(h:handle,c:caller) : bool
-  proc restrD() : (handle,capacity)fmap
-}.
-
-module type ADV_SAMPLEH(O:SAMPLE) = {
-  proc main() : bool
-}.
-
-
-
-module Esample = {
-  var handles : (handle, ccapacity)fmap
-
-  proc sampleI(h:handle) = {
-    var c;
-    c           <$ cdistr;
-    handles.[h] <- (c,I);
-  }
-
-  proc setD (h:handle, c:capacity) = {
-    handles.[h] <- (c,D);
-  }
-
-  proc in_dom(h:handle, c:caller) = {
-    return in_dom_with handles h c;
-  }
-
-  proc restrD() = {
-    return (
-      let m = NewFMap.filter (fun _ (p:ccapacity) => p.`2=D) handles in
-      NewFMap.map (fun _ (p:ccapacity) => p.`1) m);
-  }
-
-  proc get(h:handle) = {
-    var c;
-    c <$ cdistr;
-    if (!mem (dom handles) h || (oget handles.[h]).`2 = I) {
-      handles.[h] <- (c,D);
-    }
-    return (oget (handles.[h])).`1;
-  }
-
-}.
-
-
-
-
-
-
-
-
-type from, to.
-
-module type RO = {
-  proc init()     : unit
-  proc f(x : from): to
-}.
-
-module type Distinguisher(G : RO) = {
-  proc distinguish(): bool {G.f}
-}.
-
-module IND(G:RO, D:Distinguisher) = {
-  proc main(): bool = {
+  proc main1() = {
     var b;
-
-         G.init();
-    b <@ D(G).distinguish();
+    RO.init();
+    b <@ D(RO).distinguish();
     return b;
-  }  
+  }
+
+  proc main2() = {
+    var b;
+    ERO.init();
+    b <@ D(ERO).distinguish();
+    ERO.resample();
+    return b;
+  }
+
 }.
 
-abstract theory Ideal.
+equiv Eager_1_2 (D<:Distinguisher{RO}) : Eager(D).main1 ~ Eager(D).main2 : 
+  ={glob D} ==> ={res,glob RO, glob D}.
+proof.
+  proc.
+  transitivity{1} 
+    { RO.init();
+      ERO.resample();
+      b <@ D(RO).distinguish(); }
+    (={glob D} ==> ={b,RO.m,glob D})
+    (={glob D} ==> ={b,RO.m,glob D})=> //.
+  + by move=> ?&mr->;exists (glob D){mr}.
+  + inline *;rcondf{2}3;2:by sim.
+    by auto=>?;rewrite restr0 dom0 elems_fset0.
+  seq 1 1: (={glob D, RO.m});1:by inline *;auto.
+  eager (H: ERO.resample(); ~ ERO.resample();: ={RO.m} ==> ={RO.m}): 
+        (={glob D, RO.m}) => //;1:by sim.
+  eager proc H (={RO.m}) => //;try sim.
+  + by apply eager_init. + by apply eager_get. + by apply eager_set. 
+  + by apply eager_sample. + by apply eager_in_dom. + by apply eager_restrK.
+qed.
 
-  op sample : from -> to distr.
-
-  module RO = {
-    var m : (from, to) fmap
-  
-    proc init() : unit = {
-      m <- map0;
-    }
-  
-    proc f(x : from) : to = {
-      var rd;
-      rd <$ sample x;
-      if (! mem (dom m) x) m.[x] <- rd;
-      return oget m.[x];
-    }
-  }.
-
-  section LL. 
-
-    axiom sample_ll : forall x, Distr.weight (sample x) = 1%r.
-
-    lemma f_ll : phoare[RO.f : true ==> true] = 1%r. 
-    proof. proc;auto;progress;apply sample_ll. qed.
-  
-  end section LL.
- 
-end Ideal.
-
-
-abstract theory GenIdeal.
-
-  clone include Ideal. 
-  axiom sample_ll : forall x, Distr.weight (sample x) = 1%r.
-
-  op RO_dom : from fset.
-
-  module ERO = {
-    proc sample() = {
-      var work;
-      work <- RO_dom;
-      while (work <> fset0) {
-        RO.f(pick work);
-        work = work `\` fset1 (pick work);
-      }
-    }
-
-    proc init() = {
-      RO.m <- map0;
-      sample();
-    }
-
-    proc f = RO.f
-  }.
-
-  module IND_S(D:Distinguisher) = {
-    proc main(): bool = {
-      var b;
-      RO.init();
-      b <@ D(RO).distinguish();
-      ERO.sample();
-      return b;
-    }  
-  }.
-
-  section EAGER.
-
-    local lemma eager_query:
-       eager [ERO.sample(); , RO.f ~ ERO.f, ERO.sample(); :
-                 ={x,RO.m} ==> ={res,RO.m} ].
-    proof.
-      eager proc.
-      inline ERO.sample;swap{2} 4 -3.
-      seq 1 1: (={x,work,RO.m});first by sim.
-      wp;case ((mem (dom RO.m) x){1}).
-      + rnd{1}.
-        alias{1} 1 mx = oget RO.m.[x].
-        while (={work,RO.m} /\ (RO.m.[x] = Some mx){1}). 
-        + by inline *;auto;progress;smt.
-        auto;progress [- split]; rewrite sample_ll H /=;smt. 
-      case ((!mem work x){1}).
-      + swap{1} 2 -1;while (={work,x} /\ eq_except RO.m{1} RO.m{2} (fset1 x{1}) /\ 
-                             (!mem work x){1} /\ (RO.m.[x] = Some rd){2} /\ (!mem (dom RO.m) x){1}). 
-        + inline *;auto;progress [-split].
-          cut -> : mem (dom RO.m{2}) (pick work{2}) = mem (dom RO.m{1}) (pick work{2}) by rewrite !in_dom;smt.
-          smt. 
-        auto;progress [-split];rewrite !getP_eq;smt. 
-      inline RO.f.
-      transitivity{1} { rd <$ sample x;
-                        while (work <> fset0) {
-                          x0  <- pick work;
-                          rd0 <$ sample x0;
-                          if (!mem (dom RO.m) x0)
-                            RO.m.[x0] <- if x0 = x then rd else rd0;
-                          work <- work `\` fset1 (pick work);
-                        } }
-         (={x,work,RO.m} ==> ={x,RO.m})
-         ((={x,work,RO.m} /\ mem work{1} x{1}) /\ ! mem (dom RO.m{2}) x{2} ==>
-               ={x,RO.m} /\ (result = oget RO.m.[x]){2} /\ mem (dom RO.m{1}) x{1}) => //.
-      + by move=> &1 &2 H; exists RO.m{2}, x{2}, work{2}; move: H.
-      + transitivity{1} { while (work <> fset0) {
-                            x0  <- pick work;
-                            rd0 <$ sample x0;
-                            if (!mem (dom RO.m) x0) RO.m.[x0] <- rd0;
-                            work <- work `\` fset1 (pick work);
-                          }
-                          rd <$ sample x; }
-            (={x,work,RO.m} ==> ={x,RO.m})
-            (={x,work,RO.m} ==> ={x,RO.m})=> //.
-        + by move=> &1 &2 H; exists RO.m{2}, x{2}, work{2}; move: H.
-        + by sim; rnd{2}; sim : (={x,IND_Eager.H.m}); smt.
-        symmetry; eager while (H: rd <$ sample x; ~ rd <$ sample x; : ={x} ==> ={rd})=> //; sim. 
-        swap{2} 5 -4; swap [2..3] -1; case ((x = pick work){1}).
-        + by wp; rnd{2}; rnd; rnd{1}; wp; skip; smt.
-        by auto; smt.
-      + while (={x, work} /\
-               (!mem work x => mem (dom RO.m) x){1} /\
-                RO.m.[x]{2} = Some rd{1} /\
-                if (mem (dom RO.m) x){1} then ={RO.m}
-                else eq_except RO.m{1} RO.m{2} (fset1 x{1})).
-        + auto;progress; 1..9,12:smt.
-          + case ((pick work = x){2})=> pick_x; last smt.
-            subst x{2}; move: H7 H1; rewrite -neqF /eq_except=> -> /= eq_exc.
-            by apply fmapP=> x0; case (pick work{2} = x0); smt.
-        by auto; smt.
-      by auto;progress [-split];rewrite H0 /= getP_eq;smt. 
-    qed.
-
-    equiv Eager_S (D <: Distinguisher{RO}): IND_S(D).main ~ IND(ERO,D).main: ={glob D} ==> ={res,RO.m,glob D}.
-    proof.
-      proc; inline ERO.init RO.init.
-      seq 1 1: (={glob D, RO.m});first by wp. 
-      symmetry; eager (H: ERO.sample(); ~ ERO.sample();: ={RO.m} ==> ={RO.m}): 
-            (={glob D, RO.m}) => //; first by sim.
-      eager proc H (={RO.m}) => //; [by apply eager_query | by sim].
-    qed.
-
-    equiv Eager (D <: Distinguisher{RO}): IND(RO,D).main ~ IND(ERO,D).main: ={glob D} ==> ={res,glob D}.
-    proof.
-      transitivity IND_S(D).main
-          (={glob D} ==> ={res,glob D})
-          (={glob D} ==> ={res,RO.m,glob D}) => //.
-      + by progress;exists (glob D){2}.
-      + proc;inline{2} ERO.sample.
-        while{2} true (card work{2}). 
-        + move=> &m1 z;wp;call (f_ll sample_ll);auto;smt.
-        conseq (_: _ ==> ={b,glob D}) => //;[smt | by sim].
-      apply (Eager_S D).
-    qed.
-
-  end section EAGER.
-
-end GenIdeal.
-
-abstract theory FiniteIdeal.
-
-   clone include Ideal.
-   axiom sample_ll (x : from): Distr.weight (sample x) = 1%r.
-
-   op univ : from fset. 
-   axiom univP (x:from) : mem univ x.
-
-   module ERO = {
-     proc sample() = {
-       var work;
-       work <- univ;
-       while (work <> fset0) {
-         RO.f(pick work);
-         work = work `\` fset1 (pick work);
-       }
-     }
-
-     proc init() = {
-       RO.m <- map0;
-       sample();
-     }
-
-     proc f(x:from):to = { return oget RO.m.[x]; }
-  }.
-
-  module IND_S(D:Distinguisher) = {
-    proc main(): bool = {
-      var b;
-      RO.init();
-      b <@ D(RO).distinguish();
-      ERO.sample();
-      return b;
-    }  
-  }.
-
-  section EAGER.
-
-    declare module D: Distinguisher { RO }.
-
-    local clone GenIdeal as GI with 
-      op sample <- sample, 
-      op RO_dom <- univ
-      proof sample_ll by apply sample_ll.
-
-    local equiv ERO_main: 
-      IND(GI.ERO, D).main ~ IND(ERO, D).main : ={glob D} ==> ={res, glob D} /\ GI.RO.m{1} = RO.m{2}.
-    proof.
-      proc.
-      call (_:GI.RO.m{1} = RO.m{2} /\ dom RO.m{2} = univ).
-      + proc; rcondf{1} 2;auto;progress;[ by rewrite H univP | by apply sample_ll].    
-      inline *.
-      while (={work} /\ GI.RO.m{1} = RO.m{2} /\ dom RO.m{2} = univ `\` work{2});auto;smt. 
-    qed.
-
-    equiv Eager_S : IND_S(D).main ~ IND(ERO,D).main: ={glob D} ==> ={res,RO.m,glob D}.
-    proof.
-      transitivity GI.IND_S(D).main 
-          (={glob D} ==> ={res,glob D} /\ RO.m{1} = GI.RO.m{2})
-          (={glob D} ==> ={res,glob D} /\ GI.RO.m{1} = RO.m{2}) => //.
-      + by progress;exists (glob D){2}.
-      + by sim. 
-      transitivity IND(GI.ERO,D).main 
-        (={glob D} ==> ={res,glob D, GI.RO.m}) 
-        (={glob D} ==> ={res,glob D} /\ GI.RO.m{1} = RO.m{2}) => //.
-      + by progress;exists (glob D){2}.
-      + by conseq (GI.Eager_S D).
-      by apply ERO_main.     
-    qed.
-
-    equiv Eager : IND(RO, D).main ~ IND(ERO,D).main: ={glob D} ==> ={res,glob D}.
-    proof.
-      transitivity IND(GI.RO,D).main 
-          (={glob D} ==> ={res,glob D} /\ RO.m{1} = GI.RO.m{2})
-          (={glob D} ==> ={res,glob D}) => //.
-      + by progress;exists (glob D){2}.
-      + by sim. 
-      transitivity IND(GI.ERO,D).main 
-        (={glob D} ==> ={res,glob D}) 
-        (={glob D} ==> ={res,glob D}) => //.
-      + by progress;exists (glob D){2}.
-      + by conseq (GI.Eager D).
-      by conseq ERO_main.
-    qed.
-
-  end section EAGER.
-
-end FiniteIdeal.
-
-
-abstract theory RestrIdeal.
-
-  clone include Ideal.
-  axiom sample_ll (x : from): Distr.weight (sample x) = 1%r.
-
-  op test : from -> bool.
-  op univ : from fset. 
-  op dfl  : to.
-
-  axiom testP x : test x <=> mem univ x. 
-
-  module Restr (O:RO) = {
-    proc init = RO.init
-    proc f (x:from) : to = {
-      var r <- dfl;
-      if (test x) r <@ RO.f(x);
-      return r;
-    }
-  }.
-
-  module ERO = {
-     proc sample() = {
-       var work;
-       work <- univ;
-       while (work <> fset0) {
-         RO.f(pick work);
-         work = work `\` fset1 (pick work);
-       }
-     }
-
-     proc init() = {
-       RO.m <- map0;
-       sample();
-     }
-
-     proc f(x:from):to = { 
-       return (if test x then oget RO.m.[x] else dfl);
-     }
-  }.
-
-  module IND_S(D:Distinguisher) = {
-    proc main(): bool = {
-      var b;
-      RO.init();
-      b <@ D(Restr(RO)).distinguish();
-      ERO.sample();
-      return b;
-    }  
-  }.
-
-  section EAGER.
-
-    declare module D: Distinguisher { RO }.
-
-    local clone GenIdeal as GI with 
-      op sample <- sample, 
-      op RO_dom <- univ.
-
-    local module Restr' (O:RO) = {
-      proc init() = { }
-      proc f(x:from) = {  
-        var r <- dfl;
-        if (test x) r <@ O.f(x);
-        return r;
-      }
-    }.  
-        
-    local module RD (O:RO) = D(Restr'(O)).  
-
-    local equiv ERO_main: 
-      IND(GI.ERO, RD).main ~ IND(ERO, D).main : ={glob D} ==> ={res, glob D} /\ GI.RO.m{1} = RO.m{2}.
-    proof.
-      proc.
-      call (_:GI.RO.m{1} = RO.m{2} /\ dom RO.m{2} = univ).
-      + proc. 
-        case (test x{1});[ rcondt{1} 2 | rcondf{1} 2];auto;last smt ml=0.
-        by inline *;rcondf{1} 4;auto;progress;2:(by apply sample_ll);rewrite ?H0 ?H -?testP. 
-      inline *.
-      while (={work} /\ GI.RO.m{1} = RO.m{2} /\ dom RO.m{2} `|` work{2} = univ);auto;1:progress; smt.
-    qed.
-
-    equiv Eager_S : IND_S(D).main ~ IND(ERO,D).main: ={glob D} ==> ={res,RO.m,glob D}.
-    proof.
-      transitivity GI.IND_S(RD).main 
-          (={glob D} ==> ={res,glob D} /\ RO.m{1} = GI.RO.m{2})
-          (={glob D} ==> ={res,glob D} /\ GI.RO.m{1} = RO.m{2}) => //.
-      + by progress;exists (glob D){2}.
-      + by sim. 
-      transitivity IND(GI.ERO,RD).main 
-        (={glob D} ==> ={res,glob D, GI.RO.m}) 
-        (={glob D} ==> ={res,glob D} /\ GI.RO.m{1} = RO.m{2}) => //.
-      + by progress;exists (glob D){2}.
-      + by conseq (GI.Eager_S RD).
-      by apply ERO_main.     
-    qed.
-
-    equiv Eager : IND(Restr(RO), D).main ~ IND(ERO,D).main: ={glob D} ==> ={res,glob D}.
-    proof.
-      transitivity IND(GI.RO,RD).main 
-          (={glob D} ==> ={res,glob D} /\ RO.m{1} = GI.RO.m{2})
-          (={glob D} ==> ={res,glob D}) => //.
-      + by progress;exists (glob D){2}.
-      + by sim. 
-      transitivity IND(GI.ERO,RD).main 
-        (={glob D} ==> ={res,glob D}) 
-        (={glob D} ==> ={res,glob D}) => //.
-      + by progress;exists (glob D){2}.
-      + by conseq (GI.Eager RD).
-      by conseq ERO_main.
-    qed.
-
-  end section EAGER.
-
-end RestrIdeal.
+end GenEager.
